\documentclass{article}

\usepackage[a4paper, total={6.5in, 11in}]{geometry}
\setlength{\parindent}{0em}

\usepackage{latex/common}

\begin{document}

\newcommand{\under}[2]{\mathop{#1}\limits_{#2}}
\newcommand{\f}{(y_i-ax_i-b)}

\newcommand{\ff}{\f^2}
\newcommand{\fa}{\frac{\ff}{\sigma^2}}
\newcommand{\fb}{\frac{1}{2}\fa}

\newcommand{\s}{\sum\limits_{i=1}^{n}}
\newcommand{\p}[2]{\frac{\partial #1}{\partial #2}}
\newcommand{\F}{-\frac{n}{2} ln2\pi - nln\abs{\sigma} -\s \frac{1}{2} \frac{\ff}{\sigma^2}}

\newcommand{\B}[1]{\left\{\begin{aligned}#1\end{aligned}\right.}
\newcommand{\E}{\mathrm{E}}
\newcommand{\V}{\mathrm{V}}

\section{P1}

$\hat{a}, \hat{b}, \hat{\sigma^2} = \under{argmin}{a,b,\sigma^2}(\F)$

assume F = $\F$

$
\begin{aligned}
\p{F}{a} & = \p{}{a} (- \s \fb) \\
         & = -\s \p{}{a} (\fb) \\
         & = -\s \frac{1}{2} \frac{1}{\sigma^2} 2 \f (-x_i) \\
         & = \frac{n}{\sigma^2} \s x_i \f \\
\p{F}{b} & = \frac{n}{\sigma^2} \s \f
\end{aligned}
$


According to MLE, we can get the maximum at critial point of the partial derivative.

Substituting (1,2),(2,3),(4,6) into
$\B{
  \p{F}{a} = 0 \\
  \p{F}{b} = 0
}$

$\B{
  1(2-a-b) + 2(3-2a-b) + 4(6-4a-b) & = 0 \\
  (2-a-b) + (3-2a-b) + (6-4a-b)  & = 0
}$

$\hat{a}=\frac{19}{14}, \hat{b}=0.5$

$
\begin{aligned}
\p{F}{\sigma}    & = \p{}{\sigma} (-nln\abs{\sigma} - \s \fb) \\
                 & = -\frac{n}{\sigma} - \s \frac{1}{2} \ff \frac{-2}{\sigma^3} \\
                 & = -\frac{n}{\sigma} + \s \frac{\ff}{\sigma^3} \\
\p{F}{\sigma}    & = 0 \\
               0 & = -\frac{n}{\sigma} + \s \frac{\ff}{\sigma^3} \\
\frac{n}{\sigma} & = \s \frac{\ff}{\sigma^3} \\
        \sigma^2 & = \s \frac{\ff}{n} \\
  \hat{\sigma^2} & = \frac{1}{42}
\end{aligned}
$


\section{P2}

$
\begin{aligned}
\V[x] & = \E[(x-\E[x])(x-\E[x])^T] \\
      & = \E[(x-\E[x])(x^T-\E[x]^T)] \\
      & = \E[x(x^T-\E[x]^T)-\E[x](x^T-\E[x]^T)] \\
      & = \E[xx^T-x\E[x]^T-\E[x]x^T-\E[x]\E[x]^T] \\
      & = \E[xx^T]-\E[x]\E[x]^T-\E[x]\E[x^T]-\E[x]\E[x]^T \\
      & = \E[xx^T]-\E[x]\E[x^T] \\
      & = \E[xx^T]-\E[x]\E[x]^T \\
\end{aligned}
$

\newpage

\section{P3}

$\hat{x} = \under{argmin}{x} (\frac{1}{2} trace(Axx^T) - b^Tx + c)$

assume F = $\frac{1}{2} trace(Axx^T) - b^Tx + c$

Due to A is a positive definite matrix, F gets the minimum value at $\p{F}{x} = 0$.

$
\begin{aligned}
  \p{F}{x} & = \p{}{x}(\frac{1}{2} trace(Axx^T) - b^Tx + c) \\
           & = \frac{1}{2} \p{}{x}(trace((Axx^T)^T)) - b + 0 \\
           & = \frac{1}{2} \p{}{x}(trace(xx^TA^T) - b \\
           & = \p{}{xx^T}(trace(xx^TA^T) \frac{1}{2} \p{}{x}(xx^T) - b \\
           & = A \frac{1}{2} 2x - b \\
           & = Ax - b \\
  x^{k+1}  & = \alpha_k \p{F}{x} \\
  x^{k+1}  & = \alpha_k (Ax - b) \\
  \p{F}{x} & = 0 \\
       Ax  & = b \\
  \hat{x}  & = A^{-1}b
\end{aligned}
$

\end{document}
